proof/theories/Ruleset_Gen.v
@@ -19,7 +19,7 @@ Definition decls : set_decls :=
 Definition base_env : env :=
   {| e_set := fun _ => []; e_vmap := fun _ => []; e_map := fun _ => [];
      e_routes := []; e_rt := fun _ => [];
-     e_ifaddr := (fun _ => []);
+     e_ifaddr := (fun _ => []); e_ifaddr6 := (fun _ => []);
      e_limit := fun _ => 0; e_quota := fun _ => 0; e_connlimit := fun _ => 0 |}.
 
 Definition gen_env : env := env_with_sets base_env decls.
